{
 "cells": [
  {
   "cell_type": "markdown",
   "id": "5d5180d9",
   "metadata": {},
   "source": [
    "### Geometric series\n",
    "\n",
    "These are series where the difference between terms is constant.\n",
    "\n",
    "EG:\n",
    "\n",
    "$ a_n = \\frac{1}{n^2} $\n",
    "\n",
    "$ \\frac{1}{2} + \\frac{1}{4} + \\frac{1}{8} + ... + \\frac{1}{n^2} $\n",
    "\n",
    "Each term is half of the previous one, so this is a constant change, and therefore it's geometric.\n",
    "\n",
    "#### Finding the limit of $r^n$ \n",
    "\n",
    "$ a_n = r^n $\n",
    "\n",
    "$S_n =  \\sum\\limits_{n=0}^\\infty r^n $\n",
    "\n",
    "TLDR: if r < 1 then $ S_n $ tends to $\\frac{1}{1-r} $. Otherwise $ S_n $ diverges.\n",
    "\n",
    "Below, $ N - 1 $ because we start at 0, but need to still have $ N $ terms\n",
    "\n",
    "$S_N =  \\sum\\limits_{n=0}^{N-1} r^{N-1} = r^0 + r^1 + r^2 + ... r^{N-1} $\n",
    "\n",
    "$r S_N = r^1 + r^2 + r^3 + ... r^{N} $\n",
    "\n",
    "$ r S_N - S_N = (r^0 + r^1 + r^2 + ... r^{N-1}) - r^1 + r^2 + r^3 + ... r^{N} $\n",
    "\n",
    "$ r S_N - S_N = r^N - r^0 $\n",
    "\n",
    "$  S_N(r - 1) = r^N - r^0 $\n",
    "\n",
    "$  S_N(r - 1) = r^N - 1 $\n",
    "\n",
    "$  S_N = \\frac{r^N - 1}{ (r - 1) }, r \\ne 1$\n",
    "\n",
    "$  S_N = \\frac{-1( -r^N + 1)}{ -1(-r + 1) }, r \\ne 1$\n",
    "\n",
    "$  S_N = \\frac{-r^N + 1}{ -r + 1 }, r \\ne 1$\n",
    "\n",
    "BELOW, I NEED TO LEARN THE LOGIC FOR THIS.\n",
    "\n",
    "Here, read $ \\to $ as tend to, it's not an implication\n",
    "\n",
    "Also read $ |x| $ as the absolute value.\n",
    "\n",
    "Converges:\n",
    "\n",
    "$ |r| < 1 : r^N \\to 0, N \\to \\infty, S_N \\to \\frac{1}{1 - r} $\n",
    "\n",
    "Diverges:\n",
    "\n",
    "$ |r| > 1 : r^N \\to \\infty, N = \\to \\infty, S_N \\to \\infty $\n",
    "\n",
    "#### A geometric series in disguise\n",
    "\n",
    "$ S = \\frac{3}{5} + \\frac{3}{5^2} + \\frac{3}{5^3} + ... $\n",
    "\n",
    "This would need to have a 1 at the front for the former method to apply\n",
    "\n",
    "$ S = \\frac{3}{5} \\left(1 + \\frac{1}{5} + \\frac{1}{5^2} + \\frac{1}{5^3} + ... \\right)$\n",
    "\n",
    "$ \\frac{3}{5} \\sum \\limits_{n=0}^\\infty \\left(\\frac{1}{5}\\right)^n $\n",
    "\n",
    "$ r = \\frac{1}{5} $\n",
    "\n",
    "Since $ |r| < 1 $, then:\n",
    "\n",
    "$ \\sum \\limits_{n=0}^\\infty \\left(\\frac{1}{5} \\right)^n = \\frac{1}{1 - r} = \\frac{1}{1 - 1/5} = \\frac{1}{4/5} = \\frac{5}{4} $\n",
    "\n",
    "$ \\frac{3}{5}\\sum \\limits_{n=0}^\\infty \\left(\\frac{1}{5} \\right)^n = \\frac{3}{5} * \\frac{5}{4} = \\frac{3}{4}$\n",
    "\n",
    "That is therefore a finite value, and it converges\n",
    "\n",
    "#### Another one in disguise\n",
    "\n",
    "$ 0.\\dot3 = 0.3333333... $\n",
    "\n",
    "$ 0.\\dot3 = 0.3 + 0.03 + 0.003 + 0.0003 + ... $\n",
    "\n",
    "$ 0.\\dot3 = \\frac{3}{10} + \\frac{3}{100} + \\frac{3}{1000} + \\frac{3}{10,000} + ... $\n",
    "\n",
    "$ 0.\\dot3 = \\frac{3}{10^1} + \\frac{3}{10^2} + \\frac{3}{10^3} + \\frac{3}{10^4} + ... $\n",
    "\n",
    "$ 0.\\dot3 = \\frac{3}{10} \\left(1 + \\frac{3}{10^1} + \\frac{3}{10^2} + \\frac{3}{10^3} + ... \\right) $\n",
    "\n",
    "Then do the same as above."
   ]
  },
  {
   "cell_type": "code",
   "execution_count": null,
   "id": "ea36e976",
   "metadata": {},
   "outputs": [],
   "source": []
  }
 ],
 "metadata": {
  "kernelspec": {
   "display_name": "Octave",
   "language": "octave",
   "name": "octave"
  },
  "language_info": {
   "file_extension": ".m",
   "help_links": [
    {
     "text": "GNU Octave",
     "url": "https://www.gnu.org/software/octave/support.html"
    },
    {
     "text": "Octave Kernel",
     "url": "https://github.com/Calysto/octave_kernel"
    },
    {
     "text": "MetaKernel Magics",
     "url": "https://metakernel.readthedocs.io/en/latest/source/README.html"
    }
   ],
   "mimetype": "text/x-octave",
   "name": "octave",
   "version": "5.2.0"
  }
 },
 "nbformat": 4,
 "nbformat_minor": 5
}
